\section{Pliable regression splines}
\begin{frame}{Bone mineral density data}
\begin{itemize}
\item 청소년과 젊은 성인들의 골밀도 (bone mineral density) 데이터
\end{itemize}
\begin{figure}
\includegraphics[scale=0.35]{BMD}
\end{figure}
\end{frame}

\begin{frame}{Nonparametric regression model}
\begin{itemize}
\item Data :
$$
(x_1, z_1, y_1), \ldots, (x_n, z_n, y_n)
$$
\vspace{3mm}
\item Model :
$$
y_i = \mathnormal{f}(x_i, z_i) + \varepsilon_i \quad \mbox{for} \quad i = 1, \ldots, n,
$$
where $y_i \in \mathbb{R}, \; x_i \in [0,1], \; z_i = (z_{i1}, \ldots, z_{iK}) \in \mathbb{R}^K, \; E(\varepsilon_i) = 0$ and $Var(\varepsilon_i) > 0$.
\vspace{3mm}
\item Goal : 
\begin{center}
Estimate $\mathnormal{f}$ based on the given data.
\end{center}
\end{itemize}
\end{frame}

\begin{frame}{Objective function}
\begin{itemize}
\item \blue{Pliable Spline Estimator (PSE)} :

For $x \in [0,1]$ and the binary vector $ z = (z_1, \ldots, z_K)$
with length $K$, define
% Linear combination of B-splines with auxiliary binary variable :
$$
f(x, z;\theta) = \sum_{j=1}^J \beta_j B_j(x) + \sum_{j=1}^J \sum_{k=1}^K \gamma_{jk} z_k B_j(x),
$$
where 
$\theta = (\beta, \gamma_1, \ldots, \gamma_J)$ is a coefficient vector with
$\beta = (\beta_1, \ldots, \beta_J) \in \R^J$ and
$\gamma_j = (\gamma_{j1}, \ldots, \gamma_{jK}) \in \R^K$
for $j = 1, \ldots, J$. 
\vspace{3mm}
\item Residual sum of squares objective function :
$$
R(\theta) = \frac{1}{2n}\sum_{i=1}^n (y_i - f(x_i, z_i;\theta))^2
$$
\end{itemize}
\end{frame}

\begin{frame}{Coordinate descent algorithm}
\begin{itemize}
\item Univariate objective function of $\beta_j$ and $\gamma_{jk}$ :
$$
r_j (\beta_j) = R(\tilde\beta^{(-j)},\tilde\gamma_1, \ldots, \tilde\gamma_J) 
$$
and
$$
r_{jk}(\gamma_{jk}) = R \left( \tilde\beta, \tilde\gamma_1, \ldots, \tilde\gamma_{j-1},
\tilde\gamma_j^{(-k)}, \tilde\gamma_{j+1}, \ldots, \tilde\gamma_J \right)
$$
\vspace{3mm}
\item Coordinate-wise update :
$$
\tilde\beta_j \leftarrow \argmin_{\beta_j \in \R} r_j(\beta_j)
\quad\mbox{and}\quad
\tilde\gamma_{jk} \leftarrow \argmin_{\gamma_{jk} \in \R} r_{jk}(\gamma_{jk}).
$$
\end{itemize}
\end{frame}

\begin{frame}{Update $\theta = (\beta_j, \gamma_j)$ by CDA}
\begin{itemize}
\item The quadratic form of $\beta_j$
$$
r_j(\beta_j) 
= \frac{\sum_{i=1}^n B_j^2(x_i)}{2n} \left ( \beta_j - 
\frac{\sum_{i=1}^n y_{ij} B_j(x_i)}{\sum_{i=1}^n B_j^2(x_i)} \right )^2 + (\mbox{terms independent for } \beta_j)
$$
\item Update $\beta_j$
$$
\tilde\beta_j \leftarrow \frac{\sum_{i=1}^n y_{ij} B_j(x_i)}{\sum_{i=1}^n B_j^2(x_i)} 
\for j = 1, \ldots, J.
$$
\item Similarly, $r_{jk}$ can be expressed as quadratic form of $\gamma_{jk}$
\iffalse
$$
r_{jk}(\gamma_{jk})
= \frac{\sum_{i=1}^n z_{ik}^2 B_j^2(x_i)}{2n} \left \{ \gamma_{jk} - 
\frac{\sum_{i=1}^n y_{ijk} z_{ik} B_j(x_i)}{\sum_{i=1}^n z_{ik}^2 B_j^2(x_i)} \right \}^2 
+ (\mbox{terms independent for } \gamma_{jk}) 
$$
\fi
\item Update $\gamma_{jk}$
$$
\tilde\gamma_{jk} \leftarrow \frac{\sum_{i=1}^n y_{ijk} z_{ik} B_j(x_i)}{\sum_{i=1}^n z_{ik}^2 B_j^2(x_i)} 
\for j = 1, \ldots, J, \; k = 1, \ldots, K.
$$
\end{itemize}
\end{frame}